# Lezione di Matematica


$$
f:y=\frac{x^2+1}{(2x-1)(x-3)}
$$

$D$   $2x+1\neq 0\quad x\neq \frac12$
$x-3\neq 0 \quad x\neq 3$

$$
D=\left(-\infin,\frac12\right)\cup\left(\frac12,3\right)\cup\left(3,+\infin\right)
$$


1.
$$
\lim_{x\to\infin}\frac{x^2+1}{(2x-1)(x-3)}=+\frac{+\infin}{+\infin} \quad FI
$$

$$
\xrightarrow[-1=o(2x)\land 1=o(x^2)]{-3=o(x)}
$$

$$
\lim_{x\to 0})\frac{x^2}{2x}=\frac12
$$

2.

$$
\lim_{x\to\frac12^-}\frac{x^2+1}{(2x-1)(x-3)}=\frac{\frac54}{0^-\cdot\left(-\frac52\right)}=\frac{\frac54}{0^+}=+\infin
$$

3.

$$
\lim_{x\to\frac12^+}\frac{x^2+1}{(2x-1)(x-3)}=\frac{\frac54}{0^+\cdot\left(-\frac52\right)}=\frac{\frac54}{0^-}=-\infin
$$

4.
$$
\lim_{x\to3^-}\frac{x^2+1}{(2x-1)(x-3)}=\frac{10}{5\cdot 0^-}=\frac{10}{0^-}=-\infin
$$

5.
$$
\lim_{x\to3^+}\frac{x^2+1}{(2x-1)(x-3)}=\frac{10}{5\cdot 0^+}=\frac{10}{0^+}=+\infin
$$


6.
$$
\lim_{x\to+\infin}\frac{x^2+1}{(2x-1)(x-3)}=\frac{10}{5\cdot 0^+}=\frac{10}{0^+}=+\infin
$$
<!--stackedit_data:
eyJoaXN0b3J5IjpbLTIwMzU5MjM5MTVdfQ==
-->