
# Compiti di Matematica, L.5
## P. 47
### es. 318

$f(x)=(x-1)(\sqrt{x}+1)$

$f'(x)=D(\sqrt{x}+1)\cdot(x-1)+(\sqrt{x}+1)\cdot D(x-1)$

$[D(\sqrt{x})+D(1)]\cdot (x-1)+(\sqrt{x}+1)\cdot[D(x)+ D(-1)]$

$(\frac{1}{2}x^{\frac12-1}+0)\cdot(x-1)+(\sqrt{x}+1)(1+0)$

$(\frac{1}{2\sqrt{x}})(x+1)+\sqrt{x}+1$

$\frac{x-1}{2\sqrt{x}}+\sqrt{x}+1$

$\frac{x-1+2x+2\sqrt{x}}{2\sqrt{x}}$

$\frac{3x+2\sqrt{x}-1}{2\sqrt{x}}$

### 319

$f(x)=\frac{x\sqrt{x}+\sqrt[3]{x}}{x^2}$

$f'(x)=\frac{\frac{d}{dx}\left(x\sqrt{x}+\sqrt[3]{x}\right)x^2-\frac{d}{dx}\left(x^2\right)\left(x\sqrt{x}+\sqrt[3]{x}\right)}{\left(x^2\right)^2}$

$\frac{\left(\frac{3\sqrt{x}}{2}+\frac{1}{3x^{\frac{2}{3}}}\right)x^2-2x\left(x\sqrt{x}+\sqrt[3]{x}\right)}{\left(x^2\right)^2}$

$\frac{-3x\sqrt{x}-10\sqrt[3]{x}}{6x^3}$



### 323


$f(x)=x\ln(x^2+1)$

$f'(x)=\frac{d}{dx}\left(x\right)\ln \left(x^2+1\right)+\frac{d}{dx}\left(\ln \left(x^2+1\right)\right)x$

$f'(x)=1\cdot \ln \left(x^2+1\right)+\frac{2x}{x^2+1}x$

$\ln \left(x^2+1\right)+\frac{2x^2}{x^2+1}$

### 324

$f(x)=\ln|x^3-1|$

$f'(x)=\frac{1}{\left|x^3-1\right|}\frac{d}{dx}\left(\left|x^3-1\right|\right)$

$\frac{1}{\left|x^3-1\right|}\cdot \frac{3x^2\left(x^3-1\right)}{\left|x^3-1\right|}$

$\frac{3x^2}{x^3-1}$


### 325

$f(x)=\sqrt{\sin^3x}$

$f^{'}(x)=\frac{1}{2\sqrt{\sin ^3\left(x\right)}}\frac{d}{dx}\left(\sin ^3\left(x\right)\right)$

$\frac{1}{2\sqrt{\sin ^3\left(x\right)}}\cdot \:3\sin ^2\left(x\right)\cos \left(x\right)$

$\frac{3\cos \left(x\right)\sqrt{\sin \left(x\right)}}{2}$

### 328

$F(x)=e^{2x}+\sqrt[3]{e^x}$

$f^{'}(x)=\frac{d}{dx}\left(e^{2x}\right)+\frac{d}{dx}\left(\sqrt[3]{e^x}\right)$

$e^{2x}\cdot \:2+\frac{e^{\frac{x}{3}}}{3}$

### 333

$f(x)=2^{\sqrt{x}+\ln x}$

$f^{'}(x)=\frac{d}{dx}\left(e^{\left(\sqrt{x}+\ln \left(x\right)\right)\ln \left(2\right)}\right)$


$e^{\left(\sqrt{x}+\ln \left(x\right)\right)\ln \left(2\right)}\frac{d}{dx}\left(\left(\sqrt{x}+\ln \left(x\right)\right)\ln \left(2\right)\right)$

$^{\left(\sqrt{x}+\ln \left(x\right)\right)\ln \left(2\right)}\frac{\ln \left(2\right)\left(\sqrt{x}+2\right)}{2x}$

$\frac{\ln \left(2\right)\cdot \:2^{\sqrt{x}+\ln \left(x\right)-1}\left(\sqrt{x}+2\right)}{x}$
<!--stackedit_data:
eyJoaXN0b3J5IjpbNzMxNDQwNzI4XX0=
-->