# Lezione di Matematica (3° ora)

## mercoledì 28 aprile 2021, 10:00:00
$$
(\sqrt{2}-1)^x+(\sqrt{2}+1)\leq 2\\
$$
Razionalizzo
$$
(\sqrt{2}+1)\frac{(\sqrt{2}-1)}{(\sqrt{2}-1)}=\frac{2-1}{(\sqrt{2}-1)}\\
\frac{1}{\sqrt{2}-1}
$$
Risolvo
$$
(\sqrt{2}-1)^x+\frac{1}{(\sqrt{2}-1)^x}-2\leq0\\
\frac{(\sqrt{2}-1)^{2x}-2(\sqrt{2}-1)^x+1}{(\sqrt{2}-1)^x}
$$
Regola dei segni
$$
N\geq0\\
(\sqrt{2}-1)^{2x}-2(\sqrt{2}-1)^x\geq0\\
t=(\sqrt{2}-1)^x
$$
Sostituisco e risolvo
$$
t^2+2t+1=0\\
(t-1)^2=0\\
t_{1}=t_{2}=1\\
\
$$
<!--stackedit_data:
eyJoaXN0b3J5IjpbMTIwMDU0MjUxMSwtMTA3MDUzNTI0MF19
-->